correctness/RegexCorrectness/Regex/OptimizationInfo.lean
@@ -2,9 +2,11 @@ import Regex.Regex.OptimizationInfo
 import RegexCorrectness.Data.Expr.Semantics
 import RegexCorrectness.Data.Expr.Optimization
 import RegexCorrectness.Data.String
+import RegexCorrectness.Data.HashSet
 
 open Regex.Data (Expr CaptureGroups)
 open String (Iterator)
+open Std
 
 namespace Regex.OptimizationInfo
 
@@ -29,13 +31,16 @@ theorem findStart_completeness {it it' it'' : Iterator} {opt : OptimizationInfo}
   False := by
   revert lt
   fun_cases findStart opt it
-  next ch h =>
+  next cs h =>
     intro lt
-    have ne := Iterator.find_completeness v it' c.validL eqs ge lt
-    simp at ne
+    have : ¬(cs.contains it'.curr) := Iterator.find_completeness v it' c.validL eqs ge lt
     simp [eq, fromExpr] at h
-    have eq : it'.curr = ch := Expr.curr_of_captures_of_firstChar_some c h
-    exact ne eq
+    have ⟨_, h₁, h₂⟩ := h
+    have : cs.contains it'.curr := by
+      rw [← h₂]
+      simp only [HashSet.contains_toArray]
+      exact Expr.curr_of_captures_of_firstChars_some c h₁
+    contradiction
   next => exact Nat.not_lt_of_ge ge
 
 end Regex.OptimizationInfo
